src/ssa/compcert/Memtype.v
@@ -110,13 +110,13 @@ Parameter store: forall (chunk: memory_chunk) (m: mem) (b: block) (ofs: Z) (v: v
 
 Definition loadv (chunk: memory_chunk) (m: mem) (addr: val) : option val :=
   match addr with
-  | Vptr b ofs => load chunk m b (Int.signed ofs)
+  | Vptr b ofs => load chunk m b (Int.signed 31 ofs)
   | _ => None
   end.
 
 Definition storev (chunk: memory_chunk) (m: mem) (addr v: val) : option mem :=
   match addr with
-  | Vptr b ofs => store chunk m b (Int.signed ofs) v
+  | Vptr b ofs => store chunk m b (Int.signed 31 ofs) v
   | _ => None
   end.
 
@@ -225,7 +225,7 @@ Axiom valid_pointer_nonempty_perm:
   valid_pointer m b ofs = true <-> perm m b ofs Nonempty.
 Axiom valid_pointer_valid_access:
   forall m b ofs,
-  valid_pointer m b ofs = true <-> valid_access m Mint8unsigned b ofs Nonempty.
+  valid_pointer m b ofs = true <-> valid_access m (Mint 7) b ofs Nonempty.
 
 (** Each block has associated low and high bounds.  These are the bounds 
     that were given when the block was allocated.  *)
@@ -286,14 +286,11 @@ Axiom load_cast:
   forall m chunk b ofs v,
   load chunk m b ofs = Some v ->
   match chunk with
-  | Mint8signed => v = Val.sign_ext 8 v
-  | Mint8unsigned => v = Val.zero_ext 8 v
-  | Mint16signed => v = Val.sign_ext 16 v
-  | Mint16unsigned => v = Val.zero_ext 16 v
   | Mfloat32 => v = Val.singleoffloat v
   | _ => True
   end.
 
+(*
 Axiom load_int8_signed_unsigned:
   forall m b ofs,
   load Mint8signed m b ofs = option_map (Val.sign_ext 8) (load Mint8unsigned m b ofs).
@@ -301,7 +298,7 @@ Axiom load_int8_signed_unsigned:
 Axiom load_int16_signed_unsigned:
   forall m b ofs,
   load Mint16signed m b ofs = option_map (Val.sign_ext 16) (load Mint16unsigned m b ofs).
-
+*)
 
 (** ** Properties of [loadbytes]. *)
 
@@ -446,6 +443,7 @@ Axiom loadbytes_store_other:
 (** [store] is insensitive to the signedness or the high bits of
   small integer quantities. *)
 
+(*
 Axiom store_signed_unsigned_8:
   forall m b ofs v,
   store Mint8signed m b ofs v = store Mint8unsigned m b ofs v.
@@ -468,6 +466,7 @@ Axiom store_int16_sign_ext:
   forall m b ofs n,
   store Mint16signed m b ofs (Vint (Int.sign_ext 16 n)) =
   store Mint16signed m b ofs (Vint n).
+*)
 Axiom store_float32_truncate:
   forall m b ofs n,
   store Mfloat32 m b ofs (Vfloat (Float.singleoffloat n)) =
@@ -837,23 +836,23 @@ Axiom valid_pointer_inject:
 Axiom address_inject:
   forall f m1 m2 b1 ofs1 b2 delta,
   inject f m1 m2 ->
-  perm m1 b1 (Int.signed ofs1) Nonempty ->
+  perm m1 b1 (Int.signed 31 ofs1) Nonempty ->
   f b1 = Some (b2, delta) ->
-  Int.signed (Int.add ofs1 (Int.repr delta)) = Int.signed ofs1 + delta.
+  Int.signed 31 (Int.add 31 ofs1 (Int.repr 31 delta)) = Int.signed 31 ofs1 + delta.
 
 Axiom valid_pointer_inject_no_overflow:
   forall f m1 m2 b ofs b' x,
   inject f m1 m2 ->
-  valid_pointer m1 b (Int.signed ofs) = true ->
+  valid_pointer m1 b (Int.signed 31 ofs) = true ->
   f b = Some(b', x) ->
-  Int.min_signed <= Int.signed ofs + Int.signed (Int.repr x) <= Int.max_signed.
+  Int.min_signed 31 <= Int.signed 31 ofs + Int.signed 31 (Int.repr 31 x) <= Int.max_signed 31.
 
 Axiom valid_pointer_inject_val:
   forall f m1 m2 b ofs b' ofs',
   inject f m1 m2 ->
-  valid_pointer m1 b (Int.signed ofs) = true ->
+  valid_pointer m1 b (Int.signed 31 ofs) = true ->
   val_inject f (Vptr b ofs) (Vptr b' ofs') ->
-  valid_pointer m2 b' (Int.signed ofs') = true.
+  valid_pointer m2 b' (Int.signed 31 ofs') = true.
 
 Axiom inject_no_overlap:
   forall f m1 m2 b1 b2 b1' b2' delta1 delta2 ofs1 ofs2,
@@ -869,13 +868,13 @@ Axiom different_pointers_inject:
   forall f m m' b1 ofs1 b2 ofs2 b1' delta1 b2' delta2,
   inject f m m' ->
   b1 <> b2 ->
-  valid_pointer m b1 (Int.signed ofs1) = true ->
-  valid_pointer m b2 (Int.signed ofs2) = true ->
+  valid_pointer m b1 (Int.signed 31 ofs1) = true ->
+  valid_pointer m b2 (Int.signed 31 ofs2) = true ->
   f b1 = Some (b1', delta1) ->
   f b2 = Some (b2', delta2) ->
   b1' <> b2' \/
-  Int.signed (Int.add ofs1 (Int.repr delta1)) <>
-  Int.signed (Int.add ofs2 (Int.repr delta2)).
+  Int.signed 31 (Int.add 31 ofs1 (Int.repr 31 delta1)) <>
+  Int.signed 31 (Int.add 31 ofs2 (Int.repr 31 delta2)).
 
 Axiom load_inject:
   forall f m1 m2 chunk b1 ofs b2 delta v1,
@@ -951,8 +950,8 @@ Axiom alloc_left_mapped_inject:
   inject f m1 m2 ->
   alloc m1 lo hi = (m1', b1) ->
   valid_block m2 b2 ->
-  Int.min_signed <= delta <= Int.max_signed ->
-  delta = 0 \/ Int.min_signed <= low_bound m2 b2 /\ high_bound m2 b2 <= Int.max_signed ->
+  Int.min_signed 31 <= delta <= Int.max_signed 31 ->
+  delta = 0 \/ Int.min_signed 31 <= low_bound m2 b2 /\ high_bound m2 b2 <= Int.max_signed 31 ->
   (forall ofs p, lo <= ofs < hi -> perm m2 b2 (ofs + delta) p) ->
   inj_offset_aligned delta (hi-lo) ->
   (forall b ofs, 
